CFGraph/FunEval.thy
@@ -1,0 +1,106 @@
+theory Eval
+  imports CPSScheme
+begin
+
+types contour = nat
+      benv = "label \<rightharpoonup> contour"
+      closure = "lambda \<times> benv"
+
+datatype d = DI int
+           | DC closure
+           | DP prim
+           | Stop
+
+types venv = "var \<times> contour \<rightharpoonup> d"
+
+types ans = int
+
+fun evalV :: "val \<Rightarrow> benv \<Rightarrow> venv \<Rightarrow> d"
+  where "evalV (C _ i) \<beta> ve = DI i"
+  |     "evalV (P prim) \<beta> ve = DP prim"
+  |     "evalV (R _ var) \<beta> ve =
+           (case \<beta> (binder var) of
+              Some l \<Rightarrow> (case ve (var,l) of Some d \<Rightarrow> d))"
+  |     "evalV (L lam) \<beta> ve = DC (lam, \<beta>)"
+
+declare id_apply[simp del]
+function (sequential,domintros)
+         evalF :: "d \<Rightarrow> (d list) \<Rightarrow> venv \<Rightarrow> contour \<Rightarrow> ans"
+     and evalC :: "call \<Rightarrow> benv \<Rightarrow> venv \<Rightarrow> contour \<Rightarrow> ans"
+  where "evalF (DC (Lambda lab vs c, \<beta>)) as ve b
+          = (case length vs = length as of
+              True \<Rightarrow> let \<beta>' = \<beta> (lab \<mapsto> b);
+                          ve' = map_upds ve (map (\<lambda>v.(v,b)) vs) as
+                      in evalC c \<beta>' ve' b
+            )"
+  |     "evalF (DP (Plus c)) as ve b
+          = (case id as of [DI a1, DI a2, cont] \<Rightarrow>
+                   let b' = Suc b
+                   in evalF cont [DI (a1 + a2)] ve b')"
+  |     "evalF (DP (If ct cf)) [DI v, contt, contf] ve b
+          = (      if id (v \<noteq> 0) then
+                        let b' = Suc b
+                        in evalF contt [] ve b'
+                   else let b' = Suc b
+                        in evalF contf [] ve b')"
+  |     "evalF Stop as _ _
+          = (case as of [DI i] \<Rightarrow> i)"
+
+  |     "evalC (App lab f vs) \<beta> ve b
+          = (let f' = evalV f \<beta> ve;
+                 as = map (\<lambda>v. evalV v \<beta> ve) vs;
+                 b' = Suc b
+             in evalF f' as ve b')"
+  |     "evalC (Let lab ls c') \<beta> ve b
+          = (let b' = Suc b;
+                 \<beta>' = \<beta> (lab \<mapsto> b');
+                 ve' = ve ++ map_of (map (\<lambda>(v,l). ((v,b'), evalV (L l) \<beta>' ve)) ls)
+            in evalC c' \<beta>' ve' b')"
+  apply pat_completeness
+  apply auto
+done
+declare id_apply[simp]
+
+definition evalCPS :: "prog \<Rightarrow> int"
+  where "evalCPS l = (let ve = empty;
+                          \<beta> = empty;
+                          f = evalV (L l) \<beta> ve
+                      in  evalF f [Stop] ve 0)"
+
+definition eval_terminates :: "prog \<Rightarrow> bool" where
+    "eval_terminates l = (
+       let ve = empty;
+           \<beta> = empty;
+           f = evalV (L l) \<beta> ve
+       in evalF_evalC_dom (Inl (f, [Stop], ve, 0)))"
+
+lemma ex1_terminates[simp]: "eval_terminates ex1"
+unfolding eval_terminates_def
+by (auto intro!:evalF_evalC.domintros)
+
+lemma ex2_terminates[simp]: "eval_terminates ex2"
+unfolding eval_terminates_def
+by (auto intro!:evalF_evalC.domintros)
+
+(* Does not work without termination or tailrec *)
+(*
+lemma ex1_correct: "evalCPS ex1 = 0"
+unfolding evalCPS_def
+by simp
+
+lemma ex2_correct: "evalCPS ex2 = 2"
+unfolding evalCPS_def
+by simp
+*)
+
+(* These lemmas take some time, thus skipping them *)
+(*
+lemma ex3_correct: "evalCPS ex3 = 55"
+unfolding evalCPS_def
+by simp
+
+lemma ex3_terminates[simp]: "eval_terminates ex3"
+unfolding eval_terminates_def
+by (auto intro!:evalF_evalC.domintros)
+*)
+end
