CFGraph/FunExCF.thy
@@ -1,0 +1,111 @@
+theory ExCF
+  imports CPSScheme Eval
+begin
+
+(* Data types imported from Eval where possible *)
+
+types ccache = "label \<times> benv \<rightharpoonup> d"
+      ans = ccache
+
+function (sequential,domintros)
+         evalF :: "d \<Rightarrow> (d list) \<Rightarrow> venv \<Rightarrow> contour \<Rightarrow> ans"
+     and evalC :: "call \<Rightarrow> benv \<Rightarrow> venv \<Rightarrow> contour \<Rightarrow> ans"
+  where "evalF (DC (Lambda lab vs c, \<beta>)) as ve b
+          = (case length vs = length as of
+              True \<Rightarrow> let \<beta>' = \<beta> (lab \<mapsto> b);
+                          ve' = map_upds ve (map (\<lambda>v.(v,b)) vs) as
+                      in evalC c \<beta>' ve' b
+            )"
+  |     "evalF (DP (Plus c)) as ve b
+          = (case as of  [DI a1, DI a2, cont] \<Rightarrow>
+                   let b' = Suc b;
+                       \<beta>  = [c \<mapsto> b]
+                   in evalF cont [DI (a1 + a2)] ve b' ((c, \<beta>) \<mapsto> cont))"
+  |     "evalF (DP (If ct cf)) [DI v, contt, contf] ve b
+          = (      if v \<noteq> 0
+                   then let b' = Suc b;
+                            \<beta> = [ct \<mapsto> b]
+                        in evalF contt [] ve b'
+                   else let b' = Suc b;
+                            \<beta> = [cf \<mapsto> b]
+                        in evalF contf [] ve b')"
+  |     "evalF Stop as _ _
+          = (case as of [DI i] \<Rightarrow> empty)"
+
+  |     "evalC (App lab f vs) \<beta> ve b
+          = (let f' = evalV f \<beta> ve;
+                 as = map (\<lambda>v. evalV v \<beta> ve) vs;
+                 b' = Suc b
+             in evalF f' as ve b' ((lab,\<beta>) \<mapsto> f'))"
+  |     "evalC (Let lab ls c') \<beta> ve b
+          = (let b' = Suc b;
+                 \<beta>' = \<beta> (lab \<mapsto> b');
+                 ve' = ve ++ map_of (map (\<lambda>(v,l). ((v,b'), evalV (L l) \<beta>' ve)) ls)
+            in evalC c' \<beta>' ve' b')"
+  apply pat_completeness
+  apply auto
+done
+
+
+lemma ex_eval_term: "ExCF.evalF_evalC_rel = Eval.evalF_evalC_rel"
+unfolding ExCF.evalF_evalC_rel_def and Eval.evalF_evalC_rel_def
+by auto
+
+
+definition evalCPS :: "prog \<Rightarrow> ans"
+  where "evalCPS l = (let ve = empty;
+                          \<beta> = empty;
+                          f = evalV (L l) \<beta> ve
+                      in  evalF f [Stop] ve 0)"
+
+(* Variant more useful when evaluating partial functions *)
+lemmas dom_forward =
+  evalF_evalC_rel.intros(1)[THEN [2] accp_downward[of evalF_evalC_rel], OF _ eqTrueI refl refl ]
+  evalF_evalC_rel.intros(2)[THEN [2] accp_downward[of evalF_evalC_rel], OF _ refl refl refl refl refl refl refl refl]
+  evalF_evalC_rel.intros(3)[THEN [2] accp_downward[of evalF_evalC_rel], OF _ _ refl refl]
+  evalF_evalC_rel.intros(4)[THEN [2] accp_downward[of evalF_evalC_rel], OF _ _ refl refl]
+  evalF_evalC_rel.intros(5)[THEN [2] accp_downward[of evalF_evalC_rel], OF _ refl refl refl]
+  evalF_evalC_rel.intros(6)[THEN [2] accp_downward[of evalF_evalC_rel], OF _ refl refl refl]
+thm dom_forward[no_vars]
+
+thm dom_forward(1)[no_vars]
+thm evalF.psimps(1)[no_vars]
+
+lemmas dom_forward' = dom_forward(1) evalF.psimps(1)
+thm dom_forward'[no_vars]
+lemma dom_forward'': "\<lbrakk>ExCF.evalF_evalC_dom (Inl (DC (Lambda lab vs c, \<beta>), as, ve, b));
+ length vs = length as\<rbrakk>
+\<Longrightarrow> ExCF.evalF_evalC_dom
+    (Inr (c, \<beta>(lab \<mapsto> b), ve(map (\<lambda>v. (v, b)) vs [\<mapsto>] as), b)) \<and>
+ExCF.evalF (DC (Lambda lab vs c, \<beta>)) as ve b =
+(case length vs = length as of
+ True \<Rightarrow>
+   let \<beta>' = \<beta>(lab \<mapsto> b); ve' = ve(map (\<lambda>v. (v, b)) vs [\<mapsto>] as)
+   in ExCF.evalC c \<beta>' ve' b)"
+apply (insert dom_forward')
+apply auto
+done
+
+lemma correct_ex1: "evalCPS ex1 = [(2,[1 \<mapsto> 0]) \<mapsto> Stop]"
+unfolding evalCPS_def
+apply(insert "ex1_terminates")
+unfolding eval_terminates_def
+apply (simp add: ex_eval_term[THEN sym] del:evalF.psimps evalC.psimps)
+apply ((simp_all, drule dom_forward)+, simp_all)
+done
+
+
+lemma correct_ex2: "evalCPS ex2 = [(2, [1 \<mapsto> 0]) \<mapsto> DP (Plus 3), (3, [3 \<mapsto> 1]) \<mapsto> Stop]"
+unfolding evalCPS_def
+apply(insert "ex2_terminates")
+unfolding eval_terminates_def
+apply (simp add: ex_eval_term[THEN sym] del:evalF.psimps evalC.psimps)
+apply ((simp_all, drule dom_forward)+, simp_all)
+apply (rule ext)
+apply auto
+done
+
+(* Did not even try to show correctness of ex3, too large for Isabelle *)
+
+
+end
